refine/Refine.v
@@ -38,6 +38,38 @@ Module Type Adrs_Refine (Config : LLSC_Config) (Import LLSC : LLSC Config) (Impo
       snd entry <> snd entry' ->
       llsc_get_cmd nid llsc_st = LLSC.LLDone /\
       llsc_get_excl_ver nid llsc_st = v;
+    R_adrs_vl_start1 : forall nid v v' entry entry',
+      adrs_get_phase nid adrs_st = VLStart v v' ->
+      NatMap_find v adrs_st.(adrs_fsc).(fsc_val_hist) = Some entry ->
+      NatMap_find v' adrs_st.(adrs_fsc).(fsc_val_hist) = Some entry' ->
+      snd entry = snd entry' ->
+      llsc_get_excl_ver nid llsc_st = v' /\
+      exists v'', llsc_get_cmd nid llsc_st = LLSC.VLWait v'';
+    R_adrs_vl_start2 : forall nid v v' entry entry',
+      adrs_get_phase nid adrs_st = VLStart v v' ->
+      NatMap_find v adrs_st.(adrs_fsc).(fsc_val_hist) = Some entry ->
+      NatMap_find v' adrs_st.(adrs_fsc).(fsc_val_hist) = Some entry' ->
+      snd entry <> snd entry' ->
+      llsc_get_excl_ver nid llsc_st = v /\
+      exists v'', llsc_get_cmd nid llsc_st = LLSC.VLWait v'';
+    R_adrs_vl_read : forall nid v v',
+      adrs_get_phase nid adrs_st = VLRead v v' ->
+      llsc_get_excl_ver nid llsc_st = v' /\
+      exists v'', llsc_get_cmd nid llsc_st = LLSC.VLWait v'';
+    R_adrs_vl_done1 : forall nid v v' v'' entry' entry'',
+      adrs_get_phase nid adrs_st = VLDone v v' v'' ->
+      NatMap_find v' adrs_st.(adrs_fsc).(fsc_val_hist) = Some entry' ->
+      NatMap_find v'' adrs_st.(adrs_fsc).(fsc_val_hist) = Some entry'' ->
+      snd entry' = snd entry'' ->
+      llsc_get_excl_ver nid llsc_st = v' /\
+      llsc_get_cmd nid llsc_st = LLSC.VLDone true;
+    R_adrs_vl_done2 : forall nid v v' v'' entry' entry'',
+      adrs_get_phase nid adrs_st = VLDone v v' v'' ->
+      NatMap_find v' adrs_st.(adrs_fsc).(fsc_val_hist) = Some entry' ->
+      NatMap_find v'' adrs_st.(adrs_fsc).(fsc_val_hist) = Some entry'' ->
+      snd entry' <> snd entry'' ->
+      llsc_get_excl_ver nid llsc_st = v' /\
+      llsc_get_cmd nid llsc_st = LLSC.VLDone false;
     R_adrs_sc_start1 : forall nid v v' x entry entry',
       adrs_get_phase nid adrs_st = SCStart v v' x ->
       NatMap_find v adrs_st.(adrs_fsc).(fsc_val_hist) = Some entry ->
@@ -91,6 +123,11 @@ Module Type Adrs_Refine (Config : LLSC_Config) (Import LLSC : LLSC Config) (Impo
       intros NID V; destruct (Nat.eq_dec NID nid); [ subst NID; adrs_unfold; adrs_reduce; llsc_unfold; llsc_reduce; repeat rewrite NatMap_gse by auto; try discriminate | adrs_unfold; adrs_reduce; llsc_unfold; llsc_reduce; repeat rewrite NatMap_gso by auto; try apply HR ] |
       intros NID V V' Entry Entry'; destruct (Nat.eq_dec NID nid); [ subst NID; adrs_unfold; adrs_reduce; llsc_unfold; llsc_reduce; repeat rewrite NatMap_gse by auto; try discriminate | adrs_unfold; adrs_reduce; llsc_unfold; llsc_reduce; repeat rewrite NatMap_gso by auto; try apply HR ] |
       intros NID V V' Entry Entry'; destruct (Nat.eq_dec NID nid); [ subst NID; adrs_unfold; adrs_reduce; llsc_unfold; llsc_reduce; repeat rewrite NatMap_gse by auto; try discriminate | adrs_unfold; adrs_reduce; llsc_unfold; llsc_reduce; repeat rewrite NatMap_gso by auto; try apply HR ] |
+      intros NID V V' Entry Entry'; destruct (Nat.eq_dec NID nid); [ subst NID; adrs_unfold; adrs_reduce; llsc_unfold; llsc_reduce; repeat rewrite NatMap_gse by auto; try discriminate | adrs_unfold; adrs_reduce; llsc_unfold; llsc_reduce; repeat rewrite NatMap_gso by auto; try apply HR ] |
+      intros NID V V' Entry Entry'; destruct (Nat.eq_dec NID nid); [ subst NID; adrs_unfold; adrs_reduce; llsc_unfold; llsc_reduce; repeat rewrite NatMap_gse by auto; try discriminate | adrs_unfold; adrs_reduce; llsc_unfold; llsc_reduce; repeat rewrite NatMap_gso by auto; try apply HR ] |
+      intros NID V V'; destruct (Nat.eq_dec NID nid); [ subst NID; adrs_unfold; adrs_reduce; llsc_unfold; llsc_reduce; repeat rewrite NatMap_gse by auto; try discriminate | adrs_unfold; adrs_reduce; llsc_unfold; llsc_reduce; repeat rewrite NatMap_gso by auto; try apply HR ] |
+      intros NID V V' V'' Entry' Entry''; destruct (Nat.eq_dec NID nid); [ subst NID; adrs_unfold; adrs_reduce; llsc_unfold; llsc_reduce; repeat rewrite NatMap_gse by auto; try discriminate | adrs_unfold; adrs_reduce; llsc_unfold; llsc_reduce; repeat rewrite NatMap_gso by auto; try apply HR ] |
+      intros NID V V' V'' Entry' Entry''; destruct (Nat.eq_dec NID nid); [ subst NID; adrs_unfold; adrs_reduce; llsc_unfold; llsc_reduce; repeat rewrite NatMap_gse by auto; try discriminate | adrs_unfold; adrs_reduce; llsc_unfold; llsc_reduce; repeat rewrite NatMap_gso by auto; try apply HR ] |
       intros NID V V' X Entry Entry'; destruct (Nat.eq_dec NID nid); [ subst NID; adrs_unfold; adrs_reduce; llsc_unfold; llsc_reduce; repeat rewrite NatMap_gse by auto; try discriminate | adrs_unfold; adrs_reduce; llsc_unfold; llsc_reduce; repeat rewrite NatMap_gso by auto; try apply HR ] |
       intros NID V V' X Entry Entry'; destruct (Nat.eq_dec NID nid); [ subst NID; adrs_unfold; adrs_reduce; llsc_unfold; llsc_reduce; repeat rewrite NatMap_gse by auto; try discriminate | adrs_unfold; adrs_reduce; llsc_unfold; llsc_reduce; repeat rewrite NatMap_gso by auto; try apply HR ] |
       intros NID V X; destruct (Nat.eq_dec NID nid); [ subst NID; adrs_unfold; adrs_reduce; llsc_unfold; llsc_reduce; repeat rewrite NatMap_gse by auto; try discriminate | adrs_unfold; adrs_reduce; llsc_unfold; llsc_reduce; repeat rewrite NatMap_gso by auto; try apply HR ] |
@@ -130,8 +167,43 @@ Module Type Adrs_Refine (Config : LLSC_Config) (Import LLSC : LLSC Config) (Impo
       + hammer nid HR.
         intros _; eexists; reflexivity.
 
+    - (* start_vl *)
+      pose proof (adrs_ll_done_phase_prop nid _ _ _ Hval_adrs ltac:(left; apply Hpre2)) as (Hphase & _).
+      pose proof (fsc_val_hist_not_none _ v (adrs_fsc_valid _ Hval_adrs) ltac:(lia)) as Hv.
+      destruct (NatMap_find v (fsc_val_hist (adrs_fsc adrs_st))) eqn:Ev; [|contradiction]; clear Hv.
+      pose proof (fsc_val_hist_not_none _ v' (adrs_fsc_valid _ Hval_adrs) ltac:(lia)) as Hv.
+      destruct (NatMap_find v' (fsc_val_hist (adrs_fsc adrs_st))) eqn:Ev'; [|contradiction]; clear Hv.
+      destruct (Config.tag_nid_t_eq_dec (snd p) (snd p0)).
+      + exists (llsc_start_vl nid llsc_st); split.
+        * eapply reachable_step; [apply reachable_self|].
+          left; constructor; auto.
+          apply (R_adrs_ll_done1 _ _ HR _ _ _ _ _ Hpre2 Ev Ev' e).
+        * hammer nid HR.
+          -- intros Heq; injection Heq; intros ? ?; subst V V'; clear Heq.
+             intros HNID1 HNID2 HNID3.
+             pose proof (R_adrs_ll_done1 _ _ HR _ _ _ _ _ Hpre2 HNID1 HNID2 HNID3) as HR'.
+             split; [apply HR' | eexists; reflexivity].
+          -- intros Heq; injection Heq; intros ? ?; subst V V'; clear Heq.
+             intros HNID1 HNID2 HNID3.
+             pose proof (R_adrs_ll_done2 _ _ HR _ _ _ _ _ Hpre2 HNID1 HNID2 HNID3) as HR'.
+             split; [apply HR' | eexists; reflexivity].
+
+      + exists (llsc_start_vl nid llsc_st); split.
+        * eapply reachable_step; [apply reachable_self|].
+          left; constructor; auto.
+          apply (R_adrs_ll_done2 _ _ HR _ _ _ _ _ Hpre2 Ev Ev' n).
+        * hammer nid HR.
+          -- intros Heq; injection Heq; intros ? ?; subst V V'; clear Heq.
+             intros HNID1 HNID2 HNID3.
+             pose proof (R_adrs_ll_done1 _ _ HR _ _ _ _ _ Hpre2 HNID1 HNID2 HNID3) as HR'.
+             split; [apply HR' | eexists; reflexivity].
+          -- intros Heq; injection Heq; intros ? ?; subst V V'; clear Heq.
+             intros HNID1 HNID2 HNID3.
+             pose proof (R_adrs_ll_done2 _ _ HR _ _ _ _ _ Hpre2 HNID1 HNID2 HNID3) as HR'.
+             split; [apply HR' | eexists; reflexivity].
+
     - (* start_sc *)
-      pose proof (adrs_ll_done_phase_prop nid _ _ _ Hval_adrs Hpre2) as (Hphase & _).
+      pose proof (adrs_ll_done_phase_prop nid _ _ _ Hval_adrs ltac:(left; apply Hpre2)) as (Hphase & _).
       pose proof (fsc_val_hist_not_none _ v (adrs_fsc_valid _ Hval_adrs) ltac:(lia)) as Hv.
       destruct (NatMap_find v (fsc_val_hist (adrs_fsc adrs_st))) eqn:Ev; [|contradiction]; clear Hv.
       pose proof (fsc_val_hist_not_none _ v' (adrs_fsc_valid _ Hval_adrs) ltac:(lia)) as Hv.
@@ -167,7 +239,7 @@ Module Type Adrs_Refine (Config : LLSC_Config) (Import LLSC : LLSC Config) (Impo
              intros _; split; auto.
 
     - (* adrs_cl *)
-      pose proof (adrs_ll_done_phase_prop nid _ _ _ Hval_adrs Hpre2) as (Hphase & _).
+      pose proof (adrs_ll_done_phase_prop nid _ _ _ Hval_adrs ltac:(left; apply Hpre2)) as (Hphase & _).
       pose proof (fsc_val_hist_not_none _ v (adrs_fsc_valid _ Hval_adrs) ltac:(lia)) as Hv.
       destruct (NatMap_find v (fsc_val_hist (adrs_fsc adrs_st))) eqn:Ev; [|contradiction]; clear Hv.
       pose proof (fsc_val_hist_not_none _ v' (adrs_fsc_valid _ Hval_adrs) ltac:(lia)) as Hv.
@@ -218,7 +290,7 @@ Module Type Adrs_Refine (Config : LLSC_Config) (Import LLSC : LLSC Config) (Impo
       + (* equal tags *)
         exists (llsc_ret_ll nid llsc_st.(llsc_curr_ver) llsc_st); split.
         * eapply reachable_step; [apply reachable_self|].
-          right; right; econstructor.
+          right; right; right; econstructor.
           1: auto.
           1: apply Hphase2.
           rewrite (R_adrs_ver _ _ HR) in Hphase3; lia.
@@ -233,7 +305,7 @@ Module Type Adrs_Refine (Config : LLSC_Config) (Import LLSC : LLSC Config) (Impo
       + (* unequal tags *)
         exists (llsc_ret_ll nid v llsc_st); split.
         * eapply reachable_step; [apply reachable_self|].
-          right; right; econstructor.
+          right; right; right; econstructor.
           1: auto.
           1: apply Hphase2.
           rewrite (R_adrs_ver _ _ HR) in Hphase3; lia.
@@ -244,6 +316,103 @@ Module Type Adrs_Refine (Config : LLSC_Config) (Import LLSC : LLSC Config) (Impo
              intros; contradiction.
           -- intros Heq; injection Heq; intros ? ?; subst V V'; clear Heq.
              intros _ _ _; split; auto; symmetry; apply HR.
+
+    - (* vl_read *)
+      eexists llsc_st; split.
+      + apply reachable_self.
+      + hammer nid HR.
+        intros Heq; injection Heq; intros ? ?; subst V V'.
+        apply (R_adrs_vl_start1 _ _ HR _ _ _ _ _ Hpre2 Hpre3 Hpre4 Hpre5).
+
+    - (* vl_done *)
+      pose proof (adrs_ll_done_phase_prop nid _ _ _ Hval_adrs ltac:(right; right; left; apply Hpre2)) as (Hphase1 & Hphase2).
+      pose proof (fsc_val_hist_not_none _ v (adrs_fsc_valid _ Hval_adrs) ltac:(lia)) as Hv.
+      destruct (NatMap_find v (fsc_val_hist (adrs_fsc adrs_st))) eqn:Ev; [|contradiction]; clear Hv.
+      pose proof (fsc_val_hist_not_none _ v' (adrs_fsc_valid _ Hval_adrs) ltac:(lia)) as Hv'.
+      destruct (NatMap_find v' (fsc_val_hist (adrs_fsc adrs_st))) eqn:Ev'; [|contradiction]; clear Hv'.
+      pose proof (fsc_val_local_ver_not_none _ v (adrs_fsc_valid _ Hval_adrs) ltac:(lia)) as Hlv.
+      destruct (NatMap_find v (fsc_local_ver (adrs_fsc adrs_st))) eqn:Elv; [|contradiction]; clear Hlv.
+      pose proof (fsc_val_local_ver_not_none _ v' (adrs_fsc_valid _ Hval_adrs) ltac:(lia)) as Hlv'.
+      destruct (NatMap_find v' (fsc_local_ver (adrs_fsc adrs_st))) eqn:Elv'; [|contradiction]; clear Hlv'.
+      specialize (Hphase2 _ _ _ _ ltac:(reflexivity) ltac:(reflexivity) ltac:(reflexivity) ltac:(reflexivity)).
+      pose proof (adrs_vl_read_phase_prop _ _ _ _ Hval_adrs Hpre2 _ _ Ev Ev') as Heq.
+      rewrite Heq in Hphase2.
+
+      pose proof (fsc_val_hist_not_none _ (fsc_curr_ver (adrs_fsc adrs_st)) (adrs_fsc_valid _ Hval_adrs) ltac:(lia)) as Hv''.
+      destruct (NatMap_find (fsc_curr_ver (adrs_fsc adrs_st)) (fsc_val_hist (adrs_fsc adrs_st))) eqn:Ev''; [|contradiction]; clear Hv''.
+      pose proof (fsc_val_local_ver_not_none _ (fsc_curr_ver (adrs_fsc adrs_st)) (adrs_fsc_valid _ Hval_adrs) ltac:(lia)) as Hlv''.
+      destruct (NatMap_find (fsc_curr_ver (adrs_fsc adrs_st)) (fsc_local_ver (adrs_fsc adrs_st))) eqn:Elv''; [|contradiction]; clear Hlv''.
+
+      pose proof (R_adrs_vl_read _ _ HR _ _ _ Hpre2) as (HR1 & v'' & HR2).
+
+      destruct (Config.tag_nid_t_eq_dec (snd p0) (snd p1)).
+
+      + (* equal tags *)
+        exists (llsc_succ_vl nid llsc_st); split.
+        * eapply reachable_step; [apply reachable_self|].
+          right; left; econstructor.
+          1: auto.
+          1: apply HR2.
+          (* v' <= v'' <= curr_ver *)
+          pose proof (llsc_vl_wait_phase_prop1 _ _ _ Hval_llsc HR2) as Hle1.
+          pose proof (llsc_vl_wait_phase_prop2 _ _ _ Hval_llsc HR2) as Hle2.
+          rewrite HR1 in Hle2.
+          rewrite <- (R_adrs_ver _ _ HR) in Hle1.
+          (* v' = curr_ver, due to no tag reuse *)
+          assert (Heq' : v' = fsc_curr_ver (adrs_fsc adrs_st)).
+          { assert (Hneq : v' = fsc_curr_ver (adrs_fsc adrs_st) \/ v' < fsc_curr_ver (adrs_fsc adrs_st)) by lia.
+            destruct Hneq as [? | Hneq]; [auto|].
+            pose proof (fsc_local_ver_ordered _ (snd (snd p0)) v' (fsc_curr_ver (adrs_fsc adrs_st)) _ _ _ _ (adrs_fsc_valid _ Hval_adrs) ltac:(lia) Ev' Ev'' ltac:(auto) ltac:(rewrite e; auto) Elv' Elv'') as Hlt.
+            assert (Hn : n1 - n0 <= Config.n \/ n1 - n0 > Config.n) by lia.
+            destruct Hn as [Hn | Hn].
+            - pose proof (adrs_tag_no_reuse1 _ _ _ _ _ _ _ _ Hval_adrs Ev' Ev'' ltac:(reflexivity) ltac:(rewrite e; auto) Elv' Elv'' ltac:(lia) ltac:(lia) ltac:(lia)) as Hno_reuse.
+              rewrite e in Hno_reuse; contradiction.
+            - pose proof (adrs_tag_no_reuse2 _ _ _ _ _ _ _ _ Hval_adrs Hpre1 ltac:(reflexivity) ltac:(reflexivity) Ev'' ltac:(reflexivity) Elv'') as Hno_reuse.
+              rewrite <- e in Hno_reuse.
+              pose proof (read_tag_schedule_next_prop nid (adrs_get_locked_tag_local_time nid (snd (snd p0)) adrs_st) Hpre1) as Hsched.
+              specialize (Hno_reuse ltac:(lia)); clear Hsched.
+              destruct Hphase2 as (Hphase2 & _).
+              rewrite Hphase2 in Hno_reuse; contradiction.
+          }
+          lia.
+        * hammer nid HR.
+          -- intros HNID1 HNID2 HNID3 HNID4.
+             injection HNID1; intros; subst.
+             split; auto.
+          -- intros HNID1 HNID2 HNID3 HNID4.
+             injection HNID1; intros; subst.
+             rewrite Ev' in HNID2; rewrite Ev'' in HNID3.
+             injection HNID2; injection HNID3; intros; subst.
+             contradiction.
+
+      + exists (llsc_fail_vl nid llsc_st); split.
+        * eapply reachable_step; [apply reachable_self|].
+          right; left; econstructor.
+          1: auto.
+          1: apply HR2.
+          (* v' <= v'' <= curr_ver *)
+          pose proof (llsc_vl_wait_phase_prop1 _ _ _ Hval_llsc HR2) as Hle1.
+          pose proof (llsc_vl_wait_phase_prop2 _ _ _ Hval_llsc HR2) as Hle2.
+          rewrite HR1 in Hle2.
+          rewrite <- (R_adrs_ver _ _ HR) in Hle1.
+          (* Contradiction if they are equal *)
+          rewrite <- (R_adrs_ver _ _ HR).
+          rewrite HR1.
+          assert (Hneq : v' < fsc_curr_ver (adrs_fsc adrs_st) \/ v' = fsc_curr_ver (adrs_fsc adrs_st)) by lia.
+          destruct Hneq as [Hneq | Hneq]; [auto|].
+          rewrite <- Hneq in Ev''.
+          rewrite Ev' in Ev''.
+          injection Ev''; intros; subst.
+          contradiction.
+        * hammer nid HR.
+          -- intros HNID1 HNID2 HNID3 HNID4.
+             injection HNID1; intros; subst.
+             rewrite Ev' in HNID2; rewrite Ev'' in HNID3.
+             injection HNID2; injection HNID3; intros; subst.
+             contradiction.
+          -- intros HNID1 HNID2 HNID3 HNID4.
+             injection HNID1; intros; subst.
+             split; auto.
 
     - (* start_fll *)
       exists llsc_st; split.
@@ -281,20 +450,26 @@ Module Type Adrs_Refine (Config : LLSC_Config) (Import LLSC : LLSC Config) (Impo
 
       exists (llsc_succ_sc nid x llsc_st); split.
       + eapply reachable_step; [apply reachable_self|].
-        right; left; constructor; auto.
+        right; right; left; constructor; auto.
         rewrite Hphase, Hpre3.
         rewrite Heqfsc_st, (R_adrs_ver _ _ HR); auto.
       + subst fsc_st; hammer nid HR; auto.
         all: try (fold (adrs_get_phase nid adrs_st); rewrite Ephase; discriminate).
-        5: rewrite (R_adrs_ver _ _ HR); auto.
-        5: rewrite (R_adrs_ver _ _ HR); NatMap_cmp V (S (llsc_curr_ver llsc_st)); cbn; [intros Heq; inversion Heq; cbn; auto | apply HR].
-        1,2: fsc_unfold; fsc_reduce;
-             intros HNID1 HNID2 HNID3 HNID4;
-             pose proof (adrs_ll_done_phase_prop _ _ _ _ Hval_adrs HNID1) as (HNID5 & _);
+        9: rewrite (R_adrs_ver _ _ HR); auto.
+        9: rewrite (R_adrs_ver _ _ HR); NatMap_cmp V (S (llsc_curr_ver llsc_st)); cbn; [intros Heq; inversion Heq; cbn; auto | apply HR].
+        1,2,3,4,5,6: fsc_unfold; fsc_reduce;
+             intros HNID1 HNID2 HNID3;
+             pose proof (adrs_ll_done_phase_prop _ _ _ _ Hval_adrs ltac:((left; apply HNID1) || (right; left; apply HNID1) || (right; right; left; apply HNID1) || (right; right; right; eexists; apply HNID1))) as (HNID5 & _);
              rewrite NatMap_gso in HNID2 by lia;
-             rewrite NatMap_gso in HNID3 by lia.
-        1: apply (R_adrs_ll_done1 _ _ HR NID V V' Entry Entry' HNID1 HNID2 HNID3 HNID4).
-        1: apply (R_adrs_ll_done2 _ _ HR NID V V' Entry Entry' HNID1 HNID2 HNID3 HNID4).
+             try rewrite NatMap_gso in HNID3 by lia.
+        5,6: pose proof (adrs_vl_done_phase_prop _ _ _ _ _ Hval_adrs HNID1); rewrite NatMap_gso in HNID3 by lia.
+        1: apply (R_adrs_ll_done1 _ _ HR NID V V' Entry Entry' HNID1 HNID2 HNID3).
+        1: apply (R_adrs_ll_done2 _ _ HR NID V V' Entry Entry' HNID1 HNID2 HNID3).
+        1: apply (R_adrs_vl_start1 _ _ HR NID V V' Entry Entry' HNID1 HNID2 HNID3).
+        1: apply (R_adrs_vl_start2 _ _ HR NID V V' Entry Entry' HNID1 HNID2 HNID3).
+        1: apply (R_adrs_vl_done1 _ _ HR NID V V' V'' Entry' Entry'' HNID1 HNID2 HNID3).
+        1: apply (R_adrs_vl_done2 _ _ HR NID V V' V'' Entry' Entry'' HNID1 HNID2 HNID3).
+
         1,2: fsc_unfold; fsc_reduce;
              intros HNID1 HNID2 HNID3 HNID4;
              pose proof (adrs_sc_start_phase_prop _ _ _ _ _ Hval_adrs HNID1) as (HNID5 & _);
@@ -339,6 +514,54 @@ Module Type Adrs_Refine (Config : LLSC_Config) (Import LLSC : LLSC Config) (Impo
         intros _.
         apply (R_adrs_sc_scwait2 _ _ HR _ _ _ _ _ Hpre2 Hpre3).
 
+    - (* vl_fail_early *)
+      pose proof (adrs_ll_done_phase_prop nid _ _ _ Hval_adrs ltac:(right; left; apply Hpre2)) as (Hphase & _).
+      assert (Hv : v = v' \/ v < v') by lia.
+      destruct Hv as [Hv | Hv].
+      1: subst v'; rewrite Hpre3 in Hpre4; injection Hpre4; intros; subst; contradiction.
+      pose proof (R_adrs_vl_start2 _ _ HR _ _ _ _ _ Hpre2 Hpre3 Hpre4 Hpre5) as (HR1 & v'' & HR2).
+
+      exists (llsc_ret_vl nid (llsc_fail_vl nid llsc_st)); split.
+      + eapply reachable_step; [eapply reachable_step; [apply reachable_self|]|].
+        2: right; right; right; econstructor.
+        2: auto.
+        1: right; left; econstructor.
+        1: auto.
+        1: apply HR2.
+        2: llsc_unfold; llsc_reduce; rewrite NatMap_gse; auto.
+        rewrite HR1; rewrite <- (R_adrs_ver _ _ HR); lia.
+      + hammer nid HR.
+        all: intros Hphase' HNID1 HNID2 HNID3; injection Hphase'; intros; subst; clear Hphase'.
+        all: split; auto.
+        rewrite Hpre3 in HNID1; rewrite Hpre4 in HNID2; injection HNID1; injection HNID2; intros; subst.
+        contradiction.
+
+    - (* vl_fail *)
+      pose proof (R_adrs_vl_done2 _ _ HR _ _ _ _ _ _ Hpre2 Hpre3 Hpre4 Hpre5) as (HR1 & HR2).
+      exists (llsc_ret_vl nid llsc_st); split.
+      + eapply reachable_step; [apply reachable_self|].
+        right; right; right; econstructor.
+        1: auto.
+        1: apply HR2.
+      + hammer nid HR.
+        all: intros Hphase HNID1 HNID2 HNID3; injection Hphase; intros; subst V V'; split; auto.
+        pose proof (adrs_vl_done_phase_prop _ _ _ _ _ Hval_adrs Hpre2) as (_ & Hphase').
+        specialize (Hphase' _ _ HNID1 HNID2).
+        contradiction.
+
+    - (* vl_succ *)
+      pose proof (R_adrs_vl_done1 _ _ HR _ _ _ _ _ _ Hpre2 Hpre3 Hpre4 Hpre5) as (HR1 & HR2).
+      exists (llsc_ret_vl nid llsc_st); split.
+      + eapply reachable_step; [apply reachable_self|].
+        right; right; right; econstructor.
+        1: auto.
+        1: apply HR2.
+      + hammer nid HR.
+        all: intros Hphase HNID1 HNID2 HNID3; injection Hphase; intros; subst; split; auto.
+        pose proof (adrs_vl_done_phase_prop _ _ _ _ _ Hval_adrs Hpre2) as (_ & Hphase').
+        specialize (Hphase' _ _ HNID1 HNID2).
+        contradiction.
+
     - (* sc_fail *)
       pose proof (adrs_sc_ll_wait_phase_prop nid _ Hval_adrs) as (_ & Hphase & _).
       specialize (Hphase _ _ _ Hpre2) as (Hphase & _).
@@ -351,8 +574,8 @@ Module Type Adrs_Refine (Config : LLSC_Config) (Import LLSC : LLSC Config) (Impo
       exists (llsc_cl nid (llsc_fail_sc nid llsc_st)); split.
       + eapply reachable_step; [eapply reachable_step|].
         1: apply reachable_self.
-        2: right; right; econstructor.
-        1: right; left; econstructor.
+        2: right; right; right; econstructor.
+        1: right; right; left; econstructor.
         all: auto.
         1: apply HR'1.
         1: lia.
@@ -362,7 +585,7 @@ Module Type Adrs_Refine (Config : LLSC_Config) (Import LLSC : LLSC Config) (Impo
     - (* read_tag_done *)
       exists (llsc_cl nid llsc_st); split.
       + eapply reachable_step; [apply reachable_self|].
-        right; right; econstructor; auto.
+        right; right; right; econstructor; auto.
         apply (R_adrs_read_tag _ _ HR _ Hpre2).
       + hammer nid HR; auto.
   Qed.
