specs/LLSC.v
@@ -17,6 +17,8 @@ Module Type LLSC (Config : LLSC_Config).
   | Idle
   | LLWait (v : nat)
   | LLDone
+  | VLWait (v : nat)
+  | VLDone (ret : bool)
   | SCWait (x : val_t)
   | SCDone (ret : bool).
 
@@ -68,6 +70,34 @@ Module Type LLSC (Config : LLSC_Config).
     llsc_cmd := NatMap_add nid Idle st.(llsc_cmd);
   |}.
 
+  Definition llsc_start_vl (nid : nat) (st : LLSC_State) := {|
+    llsc_curr_ver := st.(llsc_curr_ver);
+    llsc_curr_excl_ver := st.(llsc_curr_excl_ver);
+    llsc_val_hist := st.(llsc_val_hist);
+    llsc_cmd := NatMap_add nid (VLWait st.(llsc_curr_ver)) st.(llsc_cmd);
+  |}.
+
+  Definition llsc_succ_vl (nid : nat) (st : LLSC_State) := {|
+    llsc_curr_ver := st.(llsc_curr_ver);
+    llsc_curr_excl_ver := st.(llsc_curr_excl_ver);
+    llsc_val_hist := st.(llsc_val_hist);
+    llsc_cmd := NatMap_add nid (VLDone true) st.(llsc_cmd);
+  |}.
+
+  Definition llsc_fail_vl (nid : nat) (st : LLSC_State) := {|
+    llsc_curr_ver := st.(llsc_curr_ver);
+    llsc_curr_excl_ver := st.(llsc_curr_excl_ver);
+    llsc_val_hist := st.(llsc_val_hist);
+    llsc_cmd := NatMap_add nid (VLDone false) st.(llsc_cmd);
+  |}.
+
+  Definition llsc_ret_vl (nid : nat) (st : LLSC_State) := {|
+    llsc_curr_ver := st.(llsc_curr_ver);
+    llsc_curr_excl_ver := st.(llsc_curr_excl_ver);
+    llsc_val_hist := st.(llsc_val_hist);
+    llsc_cmd := NatMap_add nid LLDone st.(llsc_cmd);
+  |}.
+
   Definition llsc_start_sc (nid : nat) (x : val_t) (st : LLSC_State) := {|
     llsc_curr_ver := st.(llsc_curr_ver);
     llsc_curr_excl_ver := st.(llsc_curr_excl_ver);
@@ -98,10 +128,26 @@ Module Type LLSC (Config : LLSC_Config).
       nid < Config.n ->
       llsc_get_cmd nid st = LLDone ->
       llsc_call_step st (llsc_cl nid st)
+  | llsc_call_step_vl : forall nid st,
+      nid < Config.n ->
+      llsc_get_cmd nid st = LLDone ->
+      llsc_call_step st (llsc_start_vl nid st)
   | llsc_call_step_sc : forall nid x st,
       nid < Config.n ->
       llsc_get_cmd nid st = LLDone ->
       llsc_call_step st (llsc_start_sc nid x st).
+
+  Inductive llsc_vl_step : LLSC_State -> LLSC_State -> Prop :=
+  | llsc_ret_step_vl_succ : forall nid v st,
+      nid < Config.n ->
+      llsc_get_cmd nid st = VLWait v ->
+      llsc_get_excl_ver nid st = v ->
+      llsc_vl_step st (llsc_succ_vl nid st)
+  | llsc_ret_step_vl_fail : forall nid v st,
+      nid < Config.n ->
+      llsc_get_cmd nid st = VLWait v ->
+      llsc_get_excl_ver nid st < st.(llsc_curr_ver) ->
+      llsc_vl_step st (llsc_fail_vl nid st).
 
   Inductive llsc_sc_step : LLSC_State -> LLSC_State -> Prop :=
   | llsc_ret_step_sc_succ : forall nid x st,
@@ -121,12 +167,16 @@ Module Type LLSC (Config : LLSC_Config).
       llsc_get_cmd nid st = LLWait v ->
       v <= v' <= st.(llsc_curr_ver) ->
       llsc_ret_step st (llsc_ret_ll nid v' st)
+  | llsc_ret_step_vl : forall nid b st,
+      nid < Config.n ->
+      llsc_get_cmd nid st = VLDone b ->
+      llsc_ret_step st (llsc_ret_vl nid st)
   | llsc_ret_step_sc : forall nid b st,
       nid < Config.n ->
       llsc_get_cmd nid st = SCDone b ->
       llsc_ret_step st (llsc_cl nid st).
 
-  Definition llsc_step st st' := llsc_call_step st st' \/ llsc_sc_step st st' \/ llsc_ret_step st st'.
+  Definition llsc_step st st' := llsc_call_step st st' \/ llsc_vl_step st st' \/ llsc_sc_step st st' \/ llsc_ret_step st st'.
 
   Definition llsc_sem : Semantics := {|
     s_state := LLSC_State;
@@ -137,15 +187,29 @@ Module Type LLSC (Config : LLSC_Config).
   #[local] Notation llsc_valid st := (valid_state llsc_sem st).
   #[local] Notation llsc_reachable st st' := (reachable llsc_sem st st').
 
-  Ltac llsc_unfold := unfold llsc_start_ll, llsc_ret_ll, llsc_cl, llsc_start_sc, llsc_succ_sc, llsc_fail_sc, llsc_get_excl_ver, llsc_get_cmd.
+  Ltac llsc_unfold := unfold llsc_start_ll, llsc_ret_ll, llsc_cl, llsc_start_vl, llsc_succ_vl, llsc_fail_vl, llsc_ret_vl, llsc_start_sc, llsc_succ_sc, llsc_fail_sc, llsc_get_excl_ver, llsc_get_cmd.
   Ltac llsc_reduce := cbn [llsc_curr_ver llsc_curr_excl_ver llsc_val_hist llsc_cmd].
 
   Ltac step_case Hstep :=
-    destruct Hstep as [Hstep | [Hstep | Hstep]];
-    [ destruct Hstep as [nid st Hpre1 Hpre2 | nid st Hpre1 Hpre2 | nid x st Hpre1 Hpre2] |
+    destruct Hstep as [Hstep | [Hstep | [Hstep | Hstep]]];
+    [ destruct Hstep as [nid st Hpre1 Hpre2 | nid st Hpre1 Hpre2 | nid st Hpre1 Hpre2 | nid x st Hpre1 Hpre2] |
+      destruct Hstep as [nid v st Hpre1 Hpre2 Hpre3 | nid v st Hpre1 Hpre2 Hpre3] |
       destruct Hstep as [nid x st Hpre1 Hpre2 Hpre3 | nid x st Hpre1 Hpre2 Hpre3] |
-      destruct Hstep as [nid v v' st Hpre1 Hpre2 Hpre3 | nid b st Hpre1 Hpre2]
+      destruct Hstep as [nid v v' st Hpre1 Hpre2 Hpre3 | nid b st Hpre1 Hpre2 | nid b st Hpre1 Hpre2]
     ].
+
+  Lemma llsc_excl_ver_le : forall nid st,
+    llsc_valid st ->
+    llsc_get_excl_ver nid st <= st.(llsc_curr_ver).
+  Proof.
+    intros NID st Hval.
+    induction Hval as [| st st' Hval IH Hstep].
+    - cbn; auto.
+    - step_case Hstep.
+      all: llsc_unfold; llsc_reduce; destruct (Nat.eq_dec NID nid); [subst NID; try rewrite NatMap_gse by auto; try apply IH | try rewrite NatMap_gso by auto; try apply IH].
+      all: try (fold (llsc_get_excl_ver nid st); lia).
+      all: try (fold (llsc_get_excl_ver NID st); lia).
+  Qed.
 
   Lemma llsc_ll_wait_phase_prop : forall nid v st,
     llsc_valid st ->
@@ -159,6 +223,36 @@ Module Type LLSC (Config : LLSC_Config).
       all: llsc_unfold; llsc_reduce; destruct (Nat.eq_dec NID nid); [subst NID; rewrite NatMap_gse by auto; try discriminate | rewrite NatMap_gso by auto; try apply IH].
       + intros Heq; injection Heq; intros; subst V; auto.
       + intros Heq; specialize (IH Heq); lia.
+  Qed.
+
+  Lemma llsc_vl_wait_phase_prop1 : forall nid v st,
+    llsc_valid st ->
+    llsc_get_cmd nid st = VLWait v ->
+    v <= st.(llsc_curr_ver).
+  Proof.
+    intros NID V st Hval.
+    induction Hval as [| st st' Hval IH Hstep].
+    - cbn; discriminate.
+    - step_case Hstep.
+      all: llsc_unfold; llsc_reduce; destruct (Nat.eq_dec NID nid); [subst NID; rewrite NatMap_gse by auto; try discriminate | rewrite NatMap_gso by auto; try apply IH].
+      + intros Heq; injection Heq; intros; subst V; auto.
+      + intros Heq; specialize (IH Heq); lia.
+  Qed.
+
+  Lemma llsc_vl_wait_phase_prop2 : forall nid v st,
+    llsc_valid st ->
+    llsc_get_cmd nid st = VLWait v ->
+    llsc_get_excl_ver nid st <= v.
+  Proof.
+    intros NID V st Hval.
+    induction Hval as [| st st' Hval IH Hstep].
+    - cbn; discriminate.
+    - step_case Hstep.
+      all: llsc_unfold; llsc_reduce; destruct (Nat.eq_dec NID nid); [subst NID; rewrite NatMap_gse by auto; try discriminate | rewrite NatMap_gso by auto; try apply IH].
+      + intros Hphase; injection Hphase; intros; subst V.
+        apply llsc_excl_ver_le; auto.
+      + rewrite NatMap_gso by auto.
+        auto.
   Qed.
 
 End LLSC.
